ems/ModSemE.v
@@ -1,0 +1,260 @@
+Require Import Coqlib.
+Require Export sflib.
+Require Export ITreelib.
+Require Export AList.
+Require Import Any.
+
+Set Implicit Arguments.
+
+
+Notation gname := string (only parsing). (*** convention: not capitalized ***)
+Notation mname := string (only parsing). (*** convention: capitalized ***)
+
+Section EVENTSCOMMON.
+
+  Variant eventE: Type -> Type :=
+  | Choose (X: Type): eventE X
+  | Take X: eventE X
+  | Syscall (fn: gname) (args: Any.t) (rvs: Any.t -> Prop): eventE Any.t
+  .
+
+  (* Notation "'Choose' X" := (trigger (Choose X)) (at level 50, only parsing). *)
+  (* Notation "'Take' X" := (trigger (Take X)) (at level 50, only parsing). *)
+
+  Definition triggerUB {E A} `{eventE -< E}: itree E A :=
+    v <- trigger (Take void);; match v: void with end
+  .
+
+  Definition triggerNB {E A} `{eventE -< E}: itree E A :=
+    v <- trigger (Choose void);; match v: void with end
+  .
+
+  Definition unwrapN {E X} `{eventE -< E} (x: option X): itree E X :=
+    match x with
+    | Some x => Ret x
+    | None => triggerNB
+    end.
+
+  Definition unwrapU {E X} `{eventE -< E} (x: option X): itree E X :=
+    match x with
+    | Some x => Ret x
+    | None => triggerUB
+    end.
+
+  Definition assume {E} `{eventE -< E} (P: Prop): itree E unit := trigger (Take P) ;;; Ret tt.
+  Definition guarantee {E} `{eventE -< E} (P: Prop): itree E unit := trigger (Choose P) ;;; Ret tt.
+
+  (* Notation "'unint?'" := (unwrapA <*> unint) (at level 57, only parsing). *)
+  (* Notation "'unint﹗'" := (unwrapG <*> unint) (at level 57, only parsing). *)
+  (* Notation "'Ret!' f" := (RetG f) (at level 57, only parsing). *)
+  (* Notation "'Ret?' f" := (RetA f) (at level 57, only parsing). *)
+
+  Definition unleftU {E X Y} `{eventE -< E} (xy: X + Y): itree E X :=
+    match xy with
+    | inl x => Ret x
+    | inr y => triggerUB
+    end.
+
+  Definition unleftN {E X Y} `{eventE -< E} (xy: X + Y): itree E X :=
+    match xy with
+    | inl x => Ret x
+    | inr y => triggerNB
+    end.
+
+  Definition unrightU {E X Y} `{eventE -< E} (xy: X + Y): itree E Y :=
+    match xy with
+    | inl x => triggerUB
+    | inr y => Ret y
+    end.
+
+  Definition unrightN {E X Y} `{eventE -< E} (xy: X + Y): itree E Y :=
+    match xy with
+    | inl x => triggerNB
+    | inr y => Ret y
+    end.
+
+End EVENTSCOMMON.
+
+Notation "f '?'" := (unwrapU f) (at level 9, only parsing).
+Notation "f 'ǃ'" := (unwrapN f) (at level 9, only parsing).
+Notation "(?)" := (unwrapU) (only parsing).
+Notation "(ǃ)" := (unwrapN) (only parsing).
+Goal (tt ↑↓?) = Ret tt. rewrite Any.upcast_downcast. ss. Qed.
+Goal (tt ↑↓ǃ) = Ret tt. rewrite Any.upcast_downcast. ss. Qed.
+
+
+
+
+
+
+
+Section EVENTSCOMMON.
+
+  Definition p_state: Type := (mname -> Any.t).
+
+  (*** Same as State.pure_state, but does not use "Vis" directly ***)
+  Definition pure_state {S E}: E ~> stateT S (itree E) := fun _ e s => x <- trigger e;; Ret (s, x).
+
+  Lemma unfold_interp_state: forall {E F} {S R} (h: E ~> stateT S (itree F)) (t: itree E R) (s: S),
+      interp_state h t s = _interp_state h (observe t) s.
+  Proof. i. f. apply unfold_interp_state. Qed.
+
+End EVENTSCOMMON.
+
+
+
+
+
+
+
+
+Module EventsL.
+Section EVENTSL.
+
+  Inductive callE: Type -> Type :=
+  | Call (mn: option mname) (fn: gname) (args: Any.t): callE Any.t
+  .
+
+  Inductive pE: Type -> Type :=
+  | PPut (mn: mname) (p: Any.t): pE unit
+  | PGet (mn: mname): pE Any.t
+  .
+
+  (*** TODO: we don't want to require "mname" here ***)
+  (*** use dummy mname? ***)
+  (* Definition FPut E `{rE -< E} (mn: mname) (fr: GRA): itree E unit := *)
+
+  Definition Es: Type -> Type := (callE +' pE +' eventE).
+
+  (* Inductive mdE: Type -> Type := *)
+  (* | MPut (mn: mname) (r: GRA): mdE unit *)
+  (* | MGet (mn: mname): mdE GRA *)
+  (* . *)
+
+  (* Inductive fnE: Type -> Type := *)
+  (* | FPut (r: GRA): fnE unit *)
+  (* | FGet: fnE GRA *)
+  (* | FPush: fnE unit *)
+  (* | FPop: fnE unit *)
+  (* . *)
+
+
+
+
+
+
+  (********************************************************************)
+  (*************************** Interpretation *************************)
+  (********************************************************************)
+
+  Definition handle_pE {E}: pE ~> stateT p_state (itree E) :=
+    fun _ e mps =>
+      match e with
+      | PPut mn p => Ret (update mps mn p, tt)
+      | PGet mn => Ret (mps, mps mn)
+      end.
+  Definition interp_pE {E}: itree (pE +' E) ~> stateT p_state (itree E) :=
+    (* State.interp_state (case_ ((fun _ e s0 => resum_itr (handle_pE e s0)): _ ~> stateT _ _) State.pure_state). *)
+    State.interp_state (case_ handle_pE pure_state).
+
+  (* Definition interp_Es A (prog: callE ~> itree Es) (itr0: itree Es A) (rst0: r_state) (pst0: p_state): itree eventE _ := *)
+  (*   interp_pE (interp_rE (interp_mrec prog itr0) rst0) pst0 *)
+  (* . *)
+  Definition interp_Es A (prog: callE ~> itree Es) (itr0: itree Es A) (st0: p_state): itree eventE (p_state * _)%type :=
+    '(st1, v) <- interp_pE (interp_mrec prog itr0) st0;;
+    Ret (st1, v)
+  .
+
+
+
+  Lemma interp_Es_bind
+        A B
+        (itr: itree Es A) (ktr: A -> itree Es B)
+        (prog: callE ~> itree Es)
+        st0
+    :
+      interp_Es prog (v <- itr ;; ktr v) st0 =
+      '(st1, v) <- interp_Es prog (itr) st0 ;; interp_Es prog (ktr v) st1
+  .
+  Proof. unfold interp_Es, interp_pE. des_ifs. grind. Qed.
+
+  Lemma interp_Es_tau
+        (prog: callE ~> itree Es)
+        A
+        (itr: itree Es A)
+        st0
+    :
+      interp_Es prog (tau;; itr) st0 = tau;; interp_Es prog itr st0
+  .
+  Proof. unfold interp_Es, interp_pE. des_ifs. grind. Qed.
+
+  Lemma interp_Es_ret
+        T
+        prog st0 (v: T)
+    :
+      interp_Es prog (Ret v) st0 = Ret (st0, v)
+  .
+  Proof. unfold interp_Es, interp_pE. des_ifs. grind. Qed.
+
+  Lemma interp_Es_callE
+        p st0 T
+        (* (e: Es Σ) *)
+        (e: callE T)
+    :
+      interp_Es p (trigger e) st0 = tau;; (interp_Es p (p _ e) st0)
+  .
+  Proof. unfold interp_Es, interp_pE. des_ifs. grind. Qed.
+
+  Lemma interp_Es_pE
+        p st0
+        (* (e: Es Σ) *)
+        T
+        (e: pE T)
+    :
+      interp_Es p (trigger e) st0 =
+      '(st1, r) <- handle_pE e st0;;
+      tau;; tau;;
+      Ret (st1, r)
+  .
+  Proof.
+    unfold interp_Es, interp_pE. grind.
+  Qed.
+
+  Lemma interp_Es_eventE
+        p st0
+        (* (e: Es Σ) *)
+        T
+        (e: eventE T)
+    :
+      interp_Es p (trigger e) st0 = r <- trigger e;; tau;; tau;; Ret (st0, r)
+  .
+  Proof.
+    unfold interp_Es, interp_pE. grind.
+    unfold pure_state. grind.
+  Qed.
+
+  Lemma interp_Es_triggerUB
+        (prog: callE ~> itree Es)
+        st0
+        A
+    :
+      (interp_Es prog (triggerUB) st0: itree eventE (_ * A)) = triggerUB
+  .
+  Proof.
+    unfold interp_Es, interp_pE, pure_state, triggerUB. grind.
+  Qed.
+
+  Lemma interp_Es_triggerNB
+        (prog: callE ~> itree Es)
+        st0
+        A
+    :
+      (interp_Es prog (triggerNB) st0: itree eventE (_ * A)) = triggerNB
+  .
+  Proof.
+    unfold interp_Es, interp_pE, pure_state, triggerNB. grind.
+  Qed.
+  Opaque interp_Es.
+End EVENTSL.
+End EventsL.
+Opaque EventsL.interp_Es.
